Final implementations and polish complete, ready for PR

Micro_Rust_Std_Lib/StdLib_Result.thy
@@ -10,13 +10,16 @@ begin
 section\<open>Preamble\<close>
 
 text\<open>The following two declarations are needed for contracts where we pass a function as an argument,
-since this happens multiple times below, we're including the declarations here.\<close>
+since this is needed multiple places, we're including the declarations here.\<close>
+
 declare lift_pure_to_contract_def [crush_contracts]
 ucincl_auto lift_pure_to_contract
 
 section\<open>Core material related to the \<^emph>\<open>Result\<close> type\<close>
+
 text\<open>Methods for Result enum as part of std::result implemented here 
-based on documentation at https://doc.rust-lang.org/std/result/enum.Result.html\<close>
+based on documentation at \<^url>\<open>https://doc.rust-lang.org/std/result/enum.Result.html\<close>.
+The ordering is identical to that found on the documentation page.\<close>
 
 subsection\<open>and\<close>
 
@@ -36,13 +39,14 @@ definition result_and_contract ::  \<open>('v, 'e) result \<Rightarrow> ('v, 'e)
  ('s::{sepalg}, ('v, 'e) result, 'abort) function_contract\<close> where
   [crush_contracts]: \<open>result_and_contract self res \<equiv>
     let pre  = UNIV;
-        post = \<lambda>r. \<langle>r = (case self of Ok(_) \<Rightarrow> res | Err(k) \<Rightarrow> Err(k))\<rangle>
+        post = \<lambda>r. \<langle>r = (case self of Ok(_) \<Rightarrow> res | Err(e) \<Rightarrow> Err(e))\<rangle>
     in make_function_contract pre post\<close>
 ucincl_auto result_and_contract
 
 lemma result_and_spec [crush_specs]:
   shows \<open>\<Gamma>; result_and self res \<Turnstile>\<^sub>F result_and_contract self res\<close>
-  by (crush_boot f: result_and_def contract: result_and_contract_def) (cases self; crush_base)
+  by (crush_boot f: result_and_def contract: result_and_contract_def)
+     (cases self; crush_base)
 
 subsection\<open>and_then\<close>
 
@@ -50,22 +54,22 @@ text\<open>Takes \<^verbatim>\<open>Result\<close> and some function, if \<^verb
  pass \<^verbatim>\<open>Result\<close> to the function, otherwise return the value of \<^verbatim>\<open>Err\<close>.\<close>
 
 definition result_and_then :: \<open>('v ,'e) result \<Rightarrow> 
-('v \<Rightarrow> ('machine, ('v ,'e) result, 'abort, 'i, 'o) function_body) \<Rightarrow> 
-('machine, ('v ,'e) result, 'abort, 'i, 'o) function_body\<close> where
-  \<open>result_and_then self func \<equiv> FunctionBody \<lbrakk>
+('v \<Rightarrow> ('s, ('v ,'e) result, 'abort, 'i, 'o) function_body) \<Rightarrow> 
+('s, ('v ,'e) result, 'abort, 'i, 'o) function_body\<close> where
+  \<open>result_and_then self f \<equiv> FunctionBody \<lbrakk>
     match self {
-      Ok(v) \<Rightarrow> func(v),
+      Ok(v) \<Rightarrow> f(v),
       Err(e) \<Rightarrow> Err(e)
     }
   \<rbrakk>\<close>
 
 definition result_and_then_contract :: \<open>('v, 'e) result \<Rightarrow> ('v \<Rightarrow> ('v, 'e) result) \<Rightarrow> 
-('machine::sepalg, 'abort, 'i, 'o) striple_context \<Rightarrow>
-('v \<Rightarrow> ('machine, ('v ,'e) result, 'abort, 'i prompt, 'o prompt_output) function_body) \<Rightarrow>
-('machine, ('v ,'e) result, 'abort) function_contract\<close> where
+('s::sepalg, 'abort, 'i, 'o) striple_context \<Rightarrow>
+('v \<Rightarrow> ('s, ('v ,'e) result, 'abort, 'i prompt, 'o prompt_output) function_body) \<Rightarrow>
+('s, ('v ,'e) result, 'abort) function_contract\<close> where
   [crush_contracts]: \<open>result_and_then_contract self pure_fun \<Gamma> rust_fun \<equiv>
     let pre  = \<langle>\<forall> i. \<Gamma>; rust_fun i \<Turnstile>\<^sub>F lift_pure_to_contract (pure_fun i)\<rangle>;
-        post = \<lambda>r. \<langle>r = (case self of Err(e) \<Rightarrow> Err(e) | Ok(k) \<Rightarrow> pure_fun k)\<rangle>
+        post = \<lambda>r. \<langle>r = (case self of Err(e) \<Rightarrow> Err(e) | Ok(v) \<Rightarrow> pure_fun v)\<rangle>
     in make_function_contract pre post\<close>
 ucincl_auto result_and_then_contract
 
@@ -116,8 +120,8 @@ ucincl_auto result_as_deref_contract
 
 lemma result_as_deref_spec [crush_specs]:
   shows \<open>\<Gamma>; result_as_deref self \<Turnstile>\<^sub>F result_as_deref_contract g p self opt\<close>
-proof (crush_boot f: result_as_deref_def contract: result_as_deref_contract_def)
-qed (crush_base simp add: split: result.splits)
+  by (crush_boot f: result_as_deref_def contract: result_as_deref_contract_def)
+     (crush_base split: result.splits)
 
 end
 
@@ -128,7 +132,6 @@ of mutable references, returning the inner reference as the mutable dereference 
 
 context reference
 begin
-adhoc_overloading store_update_const \<rightleftharpoons> update_fun
 
 definition result_as_deref_mut :: \<open>('a, 'b, (('c, 'd, 'v) ref, 'e) result) ref \<Rightarrow>
     ('s, (('c, 'd, 'v) ref, ('a, 'b, 'e) ref) result, 'abort, 'i prompt, 'o prompt_output) function_body\<close> where
@@ -152,16 +155,14 @@ definition result_as_deref_mut_contract ::
     in make_function_contract pre post\<close>
 ucincl_auto result_as_deref_mut_contract
 
-no_adhoc_overloading store_update_const \<rightleftharpoons> update_fun
+lemma result_ok_focus_view_Ok:
+  shows \<open>\<down>{result_ok_focus} (Ok x) \<doteq> x\<close>
+  by (simp add: focus_view_def result_ok_focus.rep_eq make_focus_raw_via_view_modify_def)
 
 lemma result_as_deref_mut_spec [crush_specs]:
   shows \<open>\<Gamma>; result_as_deref_mut self \<Turnstile>\<^sub>F result_as_deref_mut_contract g self opt\<close>
-proof (crush_boot f: result_as_deref_mut_def contract: result_as_deref_mut_contract_def, goal_cases)
-  case 1
-  show ?case
-    proof (crush_base simp add: split: result.splits)
-    qed (simp add: focus_view_def result_ok_focus.rep_eq make_focus_raw_via_view_modify_def)
-qed
+  by (crush_boot f: result_as_deref_mut_def contract: result_as_deref_mut_contract_def)
+     (crush_base simp add: result_ok_focus_view_Ok split: result.splits)
 
 end
 
@@ -172,7 +173,6 @@ into a \<^verbatim>\<open>Result\<close> of mutable references to the \<^verbati
 
 context reference
 begin       
-adhoc_overloading store_update_const \<rightleftharpoons> update_fun
 
 definition result_as_mut :: \<open>('a, 'b, ('v, 'e) result) ref \<Rightarrow>
     ('s, (('a, 'b, 'v) ref, ('a, 'b, 'e) ref) result, 'abort, 'i prompt, 'o prompt_output) function_body\<close> where
@@ -185,21 +185,19 @@ definition result_as_mut :: \<open>('a, 'b, ('v, 'e) result) ref \<Rightarrow>
 
 definition result_as_mut_contract :: \<open>'b \<Rightarrow> ('a, 'b, ('v, 'e) result) ref
      \<Rightarrow> ('v, 'e) result \<Rightarrow> ('s::{sepalg}, (('a, 'b, 'v) ref, ('a, 'b, 'e) ref) result, 'abort) function_contract\<close> where
-  [crush_contracts]: \<open>result_as_mut_contract g ref opt \<equiv>
-    let pre  = ref \<mapsto>\<langle>\<top>\<rangle> g\<down>opt;
-        post = \<lambda>res. ref \<mapsto>\<langle>\<top>\<rangle> g\<down>opt \<star> 
+  [crush_contracts]: \<open>result_as_mut_contract g self opt \<equiv>
+    let pre  = self \<mapsto>\<langle>\<top>\<rangle> g\<down>opt;
+        post = \<lambda>res. self \<mapsto>\<langle>\<top>\<rangle> g\<down>opt \<star> 
             \<langle>res = (case opt of
-                        Ok(_)  \<Rightarrow> Ok(focus_result_ok ref)
-                      | Err(_) \<Rightarrow> Err(focus_result_err ref))\<rangle>
+                        Ok(_)  \<Rightarrow> Ok(focus_result_ok self)
+                      | Err(_) \<Rightarrow> Err(focus_result_err self))\<rangle>
     in make_function_contract pre post\<close>
 ucincl_auto result_as_mut_contract
 
 lemma result_as_mut_spec [crush_specs]:
-  shows \<open>\<Gamma>; result_as_mut ref \<Turnstile>\<^sub>F result_as_mut_contract g ref opt\<close>
-proof (crush_boot f: result_as_mut_def contract: result_as_mut_contract_def)
-qed (crush_base simp add: result_is_ok_def split: result.splits)
-
-no_adhoc_overloading store_update_const \<rightleftharpoons> update_fun
+  shows \<open>\<Gamma>; result_as_mut self \<Turnstile>\<^sub>F result_as_mut_contract g self opt\<close>
+  by (crush_boot f: result_as_mut_def contract: result_as_mut_contract_def)
+     (crush_base split: result.splits)
 
 end
 
@@ -233,12 +231,13 @@ ucincl_auto result_as_ref_contract
 
 lemma result_as_ref_spec [crush_specs]:
   shows \<open>\<Gamma>; result_as_ref self \<Turnstile>\<^sub>F result_as_ref_contract g p self opt\<close>
-proof (crush_boot f: result_as_ref_def contract: result_as_ref_contract_def)
-qed (crush_base simp add: result_is_ok_def split: result.splits)
+  by (crush_boot f: result_as_ref_def contract: result_as_ref_contract_def)
+     (crush_base split: result.splits)
 
 end
 
 subsection\<open>cloned\<close>
+
 text\<open>Takes a \<^verbatim>\<open>Result\<close> type with a shared reference (ro_ref) in the \<^verbatim>\<open>ok\<close> constructor and returns a
  \<^verbatim>\<open>Result\<close> type with simply the value of the reference in the \<^verbatim>\<open>ok\<close> constructor.\<close>
 
@@ -259,24 +258,26 @@ definition result_cloned_contract ::
    (('a, 'b, 'v) ro_ref, 'e) result \<Rightarrow>
    ('s::{sepalg}, ('v, 'e) result, 'abort) function_contract\<close> where
   [crush_contracts]: \<open>result_cloned_contract g p r v self \<equiv>
-    let pre  = (unsafe_ref_from_ro_ref r) \<mapsto>\<langle>p\<rangle> g\<down>v \<star> \<langle>self = Ok (r)\<rangle>;
-        post = \<lambda>res. (unsafe_ref_from_ro_ref r) \<mapsto>\<langle>p\<rangle> g\<down>v \<star> \<langle>res = Ok (v)\<rangle>
+    let pre  = \<langle>self = Ok (r)\<rangle> \<star> (unsafe_ref_from_ro_ref r) \<mapsto>\<langle>p\<rangle> g\<down>v;
+        post = \<lambda>res. \<langle>res = Ok (v)\<rangle> \<star> (unsafe_ref_from_ro_ref r) \<mapsto>\<langle>p\<rangle> g\<down>v
     in make_function_contract pre post\<close>
 ucincl_auto result_cloned_contract
 
 lemma result_cloned_spec [crush_specs]:
   shows \<open>\<Gamma>; result_cloned self \<Turnstile>\<^sub>F result_cloned_contract g p r v self\<close>
-  by (crush_boot f: result_cloned_def contract: result_cloned_contract_def) crush_base
+  by (crush_boot f: result_cloned_def contract: result_cloned_contract_def) 
+     (crush_base)
 
 end
 
 subsection\<open>copied\<close>
+
 text\<open>Identical to cloned for the purposes of use in µRust\<close>
 
 subsection\<open>err\<close>
 
-text\<open>Converts a \<^verbatim>\<open>Result\<close> type into a \<^verbatim>\<open>Option\<close> type where only the err constructor 
-is kept while ok is discarded.\<close>
+text\<open>Converts a \<^verbatim>\<open>Result\<close> type into a \<^verbatim>\<open>Option\<close> type where only the \<^verbatim>\<open>Err\<close> constructor 
+is kept while \<^verbatim>\<open>Ok\<close> is discarded.\<close>
 
 definition result_err :: \<open>('v, 'e) result \<Rightarrow> ('s, 'e option, 'abort, 'i, 'o) function_body\<close> where
   \<open>result_err self \<equiv> FunctionBody \<lbrakk>
@@ -295,10 +296,8 @@ ucincl_auto result_err_contract
 
 lemma result_err_spec [crush_specs]:
   shows \<open>\<Gamma>; result_err res \<Turnstile>\<^sub>F result_err_contract res\<close>
-  apply (crush_boot f: result_err_def contract: result_err_contract_def)
-  apply (cases res)
-  apply crush_base
-  done
+  by (crush_boot f: result_err_def contract: result_err_contract_def)
+     (crush_base split: result.splits)
 
 subsection\<open>expect\<close>
 
@@ -324,7 +323,7 @@ ucincl_auto result_expect_contract
 lemma result_expect_spec [crush_specs]:
   shows \<open>\<Gamma>; result_expect res m \<Turnstile>\<^sub>F result_expect_contract res v\<close>
   by (crush_boot f: result_expect_def contract: result_expect_contract_def)
-     (crush_base split!: result.splits)
+     (crush_base split: result.splits)
 
 subsection\<open>expect_err\<close>
 
@@ -349,9 +348,10 @@ ucincl_auto result_expect_err_contract
 lemma result_expect_err_spec [crush_specs]:
   shows \<open>\<Gamma>; result_expect_err res m \<Turnstile>\<^sub>F result_expect_err_contract res e\<close>
   by (crush_boot f: result_expect_err_def contract: result_expect_err_contract_def)
-     (crush_base split!: result.splits)
+     (crush_base split: result.splits)
 
 subsection\<open>flatten\<close>
+
 text\<open>Takes a type \<^verbatim>\<open>Result\<close> that contains another \<^verbatim>\<open>Result\<close> in its \<^verbatim>\<open>Ok\<close> constructor and 
 returns the inner result on the \<^verbatim>\<open>Ok\<close> branch, otherwise returns self.\<close>
 
@@ -375,10 +375,12 @@ ucincl_auto result_flatten_contract
 lemma result_flatten_spec [crush_specs]:
   shows \<open>\<Gamma>; result_flatten self \<Turnstile>\<^sub>F result_flatten_contract self\<close>
   by (crush_boot f: result_flatten_def contract: result_flatten_contract_def)
-  (crush_base split!: result.splits)
+  (crush_base split: result.splits)
 
 subsection\<open>inspect\<close>
-text\<open>Takes a type \<^verbatim>\<open>Result\<close> and a function \<close>
+
+text\<open>Applies a function to the contained value if \<^verbatim>\<open>Result\<close> is \<^verbatim>\<open>Ok\<close>,
+then returns the original \<^verbatim>\<open>Result\<close> unchanged.\<close>
 
 definition result_inspect :: \<open>('v, 'e) result \<Rightarrow> 
 ('v \<Rightarrow> ('s, 'f, 'abort, 'i, 'o) function_body) \<Rightarrow>
@@ -394,9 +396,9 @@ definition result_inspect :: \<open>('v, 'e) result \<Rightarrow>
   \<rbrakk>\<close>
 
 definition result_inspect_contract ::
-  \<open>('v, 'e) result \<Rightarrow> ('v \<Rightarrow> 'f) \<Rightarrow> ('machine::sepalg, 'abort, 'i, 'o) striple_context \<Rightarrow>
-  ('v \<Rightarrow> ('machine, 'f, 'abort, 'i prompt, 'o prompt_output) function_body) \<Rightarrow>
-  ('machine, ('v, 'e) result, 'abort) function_contract\<close> where
+  \<open>('v, 'e) result \<Rightarrow> ('v \<Rightarrow> 'f) \<Rightarrow> ('s::sepalg, 'abort, 'i, 'o) striple_context \<Rightarrow>
+  ('v \<Rightarrow> ('s, 'f, 'abort, 'i prompt, 'o prompt_output) function_body) \<Rightarrow>
+  ('s, ('v, 'e) result, 'abort) function_contract\<close> where
   [crush_contracts]: \<open>result_inspect_contract self pure_fun \<Gamma> rust_fun \<equiv>
     let pre  = \<langle>\<forall> i. \<Gamma>; rust_fun i \<Turnstile>\<^sub>F lift_pure_to_contract (pure_fun i)\<rangle>;
         post = \<lambda>r. \<langle>r = self\<rangle>
@@ -419,7 +421,9 @@ proof (crush_boot f: result_inspect_def contract: result_inspect_contract_def, g
 qed
 
 subsection\<open>inspect_err\<close>
-text\<open>Takes a type \<^verbatim>\<open>Result\<close> and a function \<close>
+
+text\<open>Applies a function to the contained error if \<^verbatim>\<open>Result\<close> is \<^verbatim>\<open>Err\<close>,
+then returns the original \<^verbatim>\<open>Result\<close> unchanged.\<close>
 
 definition result_inspect_err :: \<open>('v, 'e) result \<Rightarrow> 
 ('e \<Rightarrow> ('s, 'f, 'abort, 'i, 'o) function_body) \<Rightarrow>
@@ -435,9 +439,9 @@ definition result_inspect_err :: \<open>('v, 'e) result \<Rightarrow>
   \<rbrakk>\<close>
 
 definition result_inspect_err_contract ::
-  \<open>('v, 'e) result \<Rightarrow> ('e \<Rightarrow> 'f) \<Rightarrow> ('machine::sepalg, 'abort, 'i, 'o) striple_context \<Rightarrow>
-  ('e \<Rightarrow> ('machine, 'f, 'abort, 'i prompt, 'o prompt_output) function_body) \<Rightarrow>
-  ('machine, ('v, 'e) result, 'abort) function_contract\<close> where
+  \<open>('v, 'e) result \<Rightarrow> ('e \<Rightarrow> 'f) \<Rightarrow> ('s::sepalg, 'abort, 'i, 'o) striple_context \<Rightarrow>
+  ('e \<Rightarrow> ('s, 'f, 'abort, 'i prompt, 'o prompt_output) function_body) \<Rightarrow>
+  ('s, ('v, 'e) result, 'abort) function_contract\<close> where
   [crush_contracts]: \<open>result_inspect_err_contract self pure_fun \<Gamma> rust_fun \<equiv>
     let pre  = \<langle>\<forall> i. \<Gamma>; rust_fun i \<Turnstile>\<^sub>F lift_pure_to_contract (pure_fun i)\<rangle>;
         post = \<lambda>r. \<langle>r = self\<rangle>
@@ -460,12 +464,14 @@ proof (crush_boot f: result_inspect_err_def contract: result_inspect_err_contrac
 qed
 
 subsection\<open>into_err\<close>
-text\<open>Something\<close>
+
+text\<open>Returns the value inside the \<^verbatim>\<open>Err\<close> constructor of the \<^verbatim>\<open>Result\<close> type.
+The \<^verbatim>\<open>Ok\<close> branch is unreachable and panics.\<close>
 
 definition result_into_err :: \<open>('v, 'e) result \<Rightarrow> ('s, 'e, 'abort, 'i, 'o) function_body\<close> where
   \<open>result_into_err self \<equiv> FunctionBody \<lbrakk>
     match self {
-      Ok(_)  \<Rightarrow> panic!("This should be unreachable"),
+      Ok(_)  \<Rightarrow> panic!("result_into_err: This should be unreachable"),
       Err(e) \<Rightarrow> e
     }
   \<rbrakk>\<close>
@@ -481,16 +487,18 @@ ucincl_auto result_into_err_contract
 lemma result_into_err_spec [crush_specs]:
   shows \<open>\<Gamma>; result_into_err self \<Turnstile>\<^sub>F result_into_err_contract self e\<close>
   by (crush_boot f: result_into_err_def contract: result_into_err_contract_def)
-  (crush_base)
+     (crush_base)
 
 subsection\<open>into_ok\<close>
-text\<open>Something\<close>
+
+text\<open>Returns the value inside the \<^verbatim>\<open>Ok\<close> constructor of the \<^verbatim>\<open>Result\<close> type.
+The \<^verbatim>\<open>Err\<close> branch is unreachable and panics.\<close>
 
 definition result_into_ok :: \<open>('v, 'e) result \<Rightarrow> ('s, 'v, 'abort, 'i, 'o) function_body\<close> where
   \<open>result_into_ok self \<equiv> FunctionBody \<lbrakk>
     match self {
       Ok(v)  \<Rightarrow> v,
-      Err(_) \<Rightarrow> panic!("This should be unreachable")
+      Err(_) \<Rightarrow> panic!("result_into_ok: This should be unreachable")
     }
   \<rbrakk>\<close>
 
@@ -505,7 +513,7 @@ ucincl_auto result_into_ok_contract
 lemma result_into_ok_spec [crush_specs]:
   shows \<open>\<Gamma>; result_into_ok self \<Turnstile>\<^sub>F result_into_ok_contract self v\<close>
   by (crush_boot f: result_into_ok_def contract: result_into_ok_contract_def)
-  (crush_base)
+     (crush_base)
 
 subsection\<open>is_err\<close>
 
@@ -530,9 +538,10 @@ ucincl_auto result_is_err_contract
 lemma result_is_err_spec [crush_specs]:
   shows \<open>\<Gamma>; urust_func_result_is_err res \<Turnstile>\<^sub>F result_is_err_contract res\<close>
   by (crush_boot f: urust_func_result_is_err_def contract: result_is_err_contract_def)
-     (crush_base simp add: result_is_err_def split!: result.splits)
+     (crush_base simp add: result_is_err_def split: result.splits)
 
 subsection\<open>is_err_and\<close>
+
 text\<open>Tests whether an element of \<^verbatim>\<open>Result\<close> type is the \<^verbatim>\<open>Err\<close> constructor 
 and matches the supplied predicate.\<close>
 
@@ -546,9 +555,9 @@ definition result_is_err_and :: \<open>('v, 'e) result \<Rightarrow>
   \<rbrakk>\<close>
 
 definition result_is_err_and_contract ::
-  \<open>('v, 'e) result \<Rightarrow> ('e \<Rightarrow> bool) \<Rightarrow> ('machine::sepalg, 'abort, 'i, 'o) striple_context \<Rightarrow>
-  ('e \<Rightarrow> ('machine, bool, 'abort, 'i prompt, 'o prompt_output) function_body) \<Rightarrow>
-  ('machine, bool, 'abort) function_contract\<close> 
+  \<open>('v, 'e) result \<Rightarrow> ('e \<Rightarrow> bool) \<Rightarrow> ('s::sepalg, 'abort, 'i, 'o) striple_context \<Rightarrow>
+  ('e \<Rightarrow> ('s, bool, 'abort, 'i prompt, 'o prompt_output) function_body) \<Rightarrow>
+  ('s, bool, 'abort) function_contract\<close> 
   where [crush_contracts]: \<open>result_is_err_and_contract self pure_fun \<Gamma> rust_fun \<equiv>
     let pre  = \<langle>\<forall> i. \<Gamma>; rust_fun i \<Turnstile>\<^sub>F lift_pure_to_contract (pure_fun i)\<rangle>;
         post = \<lambda>r. \<langle>r = (case self of Err(e) \<Rightarrow> (pure_fun e) | Ok(v) \<Rightarrow> False)\<rangle>
@@ -593,9 +602,10 @@ ucincl_auto result_is_ok_contract
 lemma result_is_ok_spec [crush_specs]:
   shows \<open>\<Gamma>; urust_func_result_is_ok res \<Turnstile>\<^sub>F result_is_ok_contract res\<close>
   by (crush_boot f: urust_func_result_is_ok_def contract: result_is_ok_contract_def)
-     (crush_base simp add: result_is_ok_def split!: result.splits)
+     (crush_base simp add: result_is_ok_def split: result.splits)
 
 subsection\<open>is_ok_and\<close>
+
 text\<open>Tests whether an element of \<^verbatim>\<open>Result\<close> type is the \<^verbatim>\<open>Ok\<close> constructor 
 and matches the supplied predicate.\<close>
 
@@ -609,9 +619,9 @@ definition result_is_ok_and :: \<open>('v, 'e) result \<Rightarrow>
   \<rbrakk>\<close>
 
 definition result_is_ok_and_contract ::
-  \<open>('v, 'e) result \<Rightarrow> ('v \<Rightarrow> bool) \<Rightarrow> ('machine::sepalg, 'abort, 'i, 'o) striple_context \<Rightarrow>
-  ('v \<Rightarrow> ('machine, bool, 'abort, 'i prompt, 'o prompt_output) function_body) \<Rightarrow>
-  ('machine, bool, 'abort) function_contract\<close> 
+  \<open>('v, 'e) result \<Rightarrow> ('v \<Rightarrow> bool) \<Rightarrow> ('s::sepalg, 'abort, 'i, 'o) striple_context \<Rightarrow>
+  ('v \<Rightarrow> ('s, bool, 'abort, 'i prompt, 'o prompt_output) function_body) \<Rightarrow>
+  ('s, bool, 'abort) function_contract\<close> 
   where [crush_contracts]: \<open>result_is_ok_and_contract self pure_fun \<Gamma> rust_fun \<equiv>
     let pre  = \<langle>\<forall> i. \<Gamma>; rust_fun i \<Turnstile>\<^sub>F lift_pure_to_contract (pure_fun i)\<rangle>;
         post = \<lambda>r. \<langle>r = (case self of Err(e) \<Rightarrow> False | Ok(v) \<Rightarrow> (pure_fun v))\<rangle>
@@ -657,6 +667,7 @@ lemma result_iter_spec [crush_specs]:
   by (crush_boot f: result_iter_def contract: result_iter_contract_def) crush_base
 
 subsection\<open>iter_mut\<close>
+
 text\<open>Returns a mutable iterator over the possibly contained value, yielding \<^verbatim>\<open>Ok\<close>'s payload as a
 mutable reference to the single element, or nothing for \<^verbatim>\<open>Err\<close>.\<close>
 
@@ -685,41 +696,41 @@ ucincl_auto result_iter_mut_contract
 
 lemma result_iter_mut_spec [crush_specs]:
   shows \<open>\<Gamma>; result_iter_mut self \<Turnstile>\<^sub>F result_iter_mut_contract g self opt\<close>
-proof (crush_boot f: result_iter_mut_def contract: result_iter_mut_contract_def)
-qed (crush_base simp add: fun_literal_def split: result.splits)
+  by (crush_boot f: result_iter_mut_def contract: result_iter_mut_contract_def)
+     (crush_base split: result.splits)
 
 end
 
 subsection\<open>map\<close>
+
 text\<open>Maps a function to the \<^verbatim>\<open>Ok\<close> constructor of the \<^verbatim>\<open>Result\<close> type.\<close>
 
-definition result_map :: \<open>('a, 'e) result \<Rightarrow> ('a \<Rightarrow> ('machine, 'f, 'abort, 'i, 'o) function_body) \<Rightarrow>
-    ('machine, ('f, 'e) result, 'abort, 'i, 'o) function_body\<close> where
-  \<open>result_map x f \<equiv> FunctionBody \<lbrakk>
-     match x {
-       Ok(a)  \<Rightarrow> Ok(f(a)),
+definition result_map :: \<open>('v, 'e) result \<Rightarrow> ('v \<Rightarrow> ('s, 'f, 'abort, 'i, 'o) function_body) \<Rightarrow>
+    ('s, ('f, 'e) result, 'abort, 'i, 'o) function_body\<close> where
+  \<open>result_map self f \<equiv> FunctionBody \<lbrakk>
+     match self {
+       Ok(v)  \<Rightarrow> Ok(f(v)),
        Err(e) \<Rightarrow> Err(e)
      }
   \<rbrakk>\<close>
 
-definition result_map_contract :: \<open>('a, 'e) result \<Rightarrow> ('a \<Rightarrow> 'f) \<Rightarrow> 
-('machine::sepalg, 'abort, 'i, 'o) striple_context \<Rightarrow>
-('a \<Rightarrow> ('machine, 'f, 'abort, 'i prompt, 'o prompt_output) function_body) \<Rightarrow>
-('machine, ('f, 'e) result, 'abort) function_contract\<close> where
-  [crush_contracts]: \<open>result_map_contract res pure_fun \<Gamma> rust_fun \<equiv>
+definition result_map_contract :: \<open>('v, 'e) result \<Rightarrow> ('v \<Rightarrow> 'f) \<Rightarrow> 
+('s::sepalg, 'abort, 'i, 'o) striple_context \<Rightarrow>
+('v \<Rightarrow> ('s, 'f, 'abort, 'i prompt, 'o prompt_output) function_body) \<Rightarrow>
+('s, ('f, 'e) result, 'abort) function_contract\<close> where
+  [crush_contracts]: \<open>result_map_contract self pure_fun \<Gamma> rust_fun \<equiv>
     let pre  = \<langle>\<forall> i. \<Gamma>; rust_fun i \<Turnstile>\<^sub>F lift_pure_to_contract (pure_fun i)\<rangle>;
-        post = \<lambda>r. \<langle>r = (case res of Err(e) \<Rightarrow> Err(e) | Ok(k) \<Rightarrow> Ok(pure_fun k))\<rangle>
+        post = \<lambda>r. \<langle>r = (case self of Err(e) \<Rightarrow> Err(e) | Ok(v) \<Rightarrow> Ok(pure_fun v))\<rangle>
     in make_function_contract pre post\<close>
 ucincl_auto result_map_contract
 
-
 lemma result_map_spec [crush_specs]:
-  shows \<open>\<Gamma>; result_map res rust_fun \<Turnstile>\<^sub>F result_map_contract res pure_fun \<Gamma> rust_fun\<close>
+  shows \<open>\<Gamma>; result_map self rust_fun \<Turnstile>\<^sub>F result_map_contract self pure_fun \<Gamma> rust_fun\<close>
 proof (crush_boot f: result_map_def contract: result_map_contract_def, goal_cases)
   case 1
   note rust_fun_spec = this[THEN spec]
   show ?case
-  proof (cases res)
+  proof (cases self)
     case (Ok x1)
     then show ?thesis by (crush_base specs add: rust_fun_spec)
   next
@@ -732,33 +743,32 @@ subsection\<open>map_err\<close>
 
 text\<open>Maps a function to the \<^verbatim>\<open>Err\<close> constructor of the \<^verbatim>\<open>Result\<close> type.\<close>
 
-definition result_map_err :: \<open>('a, 'e) result \<Rightarrow> ('e \<Rightarrow> ('machine, 'f, 'abort, 'i, 'o) function_body) \<Rightarrow>
-    ('machine, ('a, 'f) result, 'abort, 'i, 'o) function_body\<close> where
-  \<open>result_map_err x f \<equiv> FunctionBody \<lbrakk>
-     match x {
-       Ok(a)  \<Rightarrow> Ok(a),
+definition result_map_err :: \<open>('v, 'e) result \<Rightarrow> ('e \<Rightarrow> ('s, 'f, 'abort, 'i, 'o) function_body) \<Rightarrow>
+    ('s, ('v, 'f) result, 'abort, 'i, 'o) function_body\<close> where
+  \<open>result_map_err self f \<equiv> FunctionBody \<lbrakk>
+     match self {
+       Ok(v)  \<Rightarrow> Ok(v),
        Err(e) \<Rightarrow> Err(f(e))
      }
   \<rbrakk>\<close>
 
-definition result_map_err_contract :: \<open>('a, 'e) result \<Rightarrow> ('e \<Rightarrow> 'f) \<Rightarrow> 
-('machine::sepalg, 'abort, 'i, 'o) striple_context \<Rightarrow>
-('e \<Rightarrow> ('machine, 'f, 'abort, 'i prompt, 'o prompt_output) function_body) \<Rightarrow>
-('machine, ('a, 'f) result, 'abort) function_contract\<close> where
-  [crush_contracts]: \<open>result_map_err_contract res pure_fun \<Gamma> rust_fun \<equiv>
+definition result_map_err_contract :: \<open>('v, 'e) result \<Rightarrow> ('e \<Rightarrow> 'f) \<Rightarrow> 
+('s::sepalg, 'abort, 'i, 'o) striple_context \<Rightarrow>
+('e \<Rightarrow> ('s, 'f, 'abort, 'i prompt, 'o prompt_output) function_body) \<Rightarrow>
+('s, ('v, 'f) result, 'abort) function_contract\<close> where
+  [crush_contracts]: \<open>result_map_err_contract self pure_fun \<Gamma> rust_fun \<equiv>
     let pre  = \<langle>\<forall> i. \<Gamma>; rust_fun i \<Turnstile>\<^sub>F lift_pure_to_contract (pure_fun i)\<rangle>;
-        post = \<lambda>r. \<langle>r = (case res of Err(e) \<Rightarrow> Err(pure_fun e) | Ok(k) \<Rightarrow> Ok(k))\<rangle>
+        post = \<lambda>r. \<langle>r = (case self of Err(e) \<Rightarrow> Err(pure_fun e) | Ok(v) \<Rightarrow> Ok(v))\<rangle>
     in make_function_contract pre post\<close>
 ucincl_auto result_map_err_contract
 
-
 lemma result_map_err_spec [crush_specs]:
-  shows \<open>\<Gamma>; result_map_err res rust_fun \<Turnstile>\<^sub>F result_map_err_contract res pure_fun \<Gamma> rust_fun\<close>
+  shows \<open>\<Gamma>; result_map_err self rust_fun \<Turnstile>\<^sub>F result_map_err_contract self pure_fun \<Gamma> rust_fun\<close>
 proof (crush_boot f: result_map_err_def contract: result_map_err_contract_def, goal_cases)
   case 1
   note rust_fun_spec = this[THEN spec]
   show ?case
-  proof (cases res)
+  proof (cases self)
     case (Ok x1)
     then show ?thesis by crush_base
   next
@@ -768,12 +778,13 @@ proof (crush_boot f: result_map_err_def contract: result_map_err_contract_def, g
 qed
 
 subsection\<open>map_or\<close>
+
 text\<open>Applies a function to the contained value if \<^verbatim>\<open>Result\<close> is \<^verbatim>\<open>Ok\<close> and returns the resulting value.
 Else, if \<^verbatim>\<open>Result\<close> is \<^verbatim>\<open>Err\<close>, returns the supplied default value.\<close>
 
 definition result_map_or :: \<open>('v, 'e) result \<Rightarrow> 'f \<Rightarrow>
-    ('v \<Rightarrow> ('machine, 'f, 'abort, 'i, 'o) function_body) \<Rightarrow>
-    ('machine, 'f, 'abort, 'i, 'o) function_body\<close> where
+    ('v \<Rightarrow> ('s, 'f, 'abort, 'i, 'o) function_body) \<Rightarrow>
+    ('s, 'f, 'abort, 'i, 'o) function_body\<close> where
   \<open>result_map_or self d f \<equiv> FunctionBody \<lbrakk>
      match self {
        Ok(v)  \<Rightarrow> f(v),
@@ -782,15 +793,14 @@ definition result_map_or :: \<open>('v, 'e) result \<Rightarrow> 'f \<Rightarrow
   \<rbrakk>\<close>
 
 definition result_map_or_contract :: \<open>('v, 'e) result \<Rightarrow> 'f \<Rightarrow> ('v \<Rightarrow> 'f) \<Rightarrow> 
-('machine::sepalg, 'abort, 'i, 'o) striple_context \<Rightarrow>
-('v \<Rightarrow> ('machine, 'f, 'abort, 'i prompt, 'o prompt_output) function_body) \<Rightarrow>
-('machine, 'f, 'abort) function_contract\<close> where
+('s::sepalg, 'abort, 'i, 'o) striple_context \<Rightarrow>
+('v \<Rightarrow> ('s, 'f, 'abort, 'i prompt, 'o prompt_output) function_body) \<Rightarrow>
+('s, 'f, 'abort) function_contract\<close> where
   [crush_contracts]: \<open>result_map_or_contract self d pure_fun \<Gamma> rust_fun \<equiv>
     let pre  = \<langle>\<forall> i. \<Gamma>; rust_fun i \<Turnstile>\<^sub>F lift_pure_to_contract (pure_fun i)\<rangle>;
         post = \<lambda>r. \<langle>r = (case self of Err(e) \<Rightarrow> d | Ok(v) \<Rightarrow> pure_fun v)\<rangle>
     in make_function_contract pre post\<close>
 ucincl_auto result_map_or_contract
-
 
 lemma result_map_or_spec [crush_specs]:
   shows \<open>\<Gamma>; result_map_or self d rust_fun \<Turnstile>\<^sub>F result_map_or_contract self d pure_fun \<Gamma> rust_fun\<close>
@@ -808,17 +818,19 @@ proof (crush_boot f: result_map_or_def contract: result_map_or_contract_def, goa
 qed
 
 subsection\<open>map_or_default\<close>
+
 text\<open>Default values are not implemented for µRust types, therefore result_map_or is the closest
 functional equivalent and should be used in place of result_map_or_default.\<close>
 
 subsection\<open>map_or_else\<close>
+
 text\<open>Applies a function to the contained value if \<^verbatim>\<open>Result\<close> is \<^verbatim>\<open>Ok\<close> and returns the resulting value.
 Else, if \<^verbatim>\<open>Result\<close> is \<^verbatim>\<open>Err\<close>, same as for \<^verbatim>\<open>Ok\<close> but with another function for the contained \<^verbatim>\<open>Err\<close> value.\<close>
 
 definition result_map_or_else :: \<open>('v, 'e) result \<Rightarrow>
-    ('e \<Rightarrow> ('machine, 'f, 'abort, 'i, 'o) function_body) \<Rightarrow>
-    ('v \<Rightarrow> ('machine, 'f, 'abort, 'i, 'o) function_body) \<Rightarrow>
-    ('machine, 'f, 'abort, 'i, 'o) function_body\<close> where
+    ('e \<Rightarrow> ('s, 'f, 'abort, 'i, 'o) function_body) \<Rightarrow>
+    ('v \<Rightarrow> ('s, 'f, 'abort, 'i, 'o) function_body) \<Rightarrow>
+    ('s, 'f, 'abort, 'i, 'o) function_body\<close> where
   \<open>result_map_or_else self d f \<equiv> FunctionBody \<lbrakk>
      match self {
        Ok(v)  \<Rightarrow> f(v),
@@ -827,17 +839,16 @@ definition result_map_or_else :: \<open>('v, 'e) result \<Rightarrow>
   \<rbrakk>\<close>
 
 definition result_map_or_else_contract :: \<open>('v, 'e) result \<Rightarrow> ('e \<Rightarrow> 'f) \<Rightarrow> ('v \<Rightarrow> 'f) \<Rightarrow> 
-('machine::sepalg, 'abort, 'i, 'o) striple_context \<Rightarrow>
-('e \<Rightarrow> ('machine, 'f, 'abort, 'i prompt, 'o prompt_output) function_body) \<Rightarrow>
-('v \<Rightarrow> ('machine, 'f, 'abort, 'i prompt, 'o prompt_output) function_body) \<Rightarrow>
-('machine, 'f, 'abort) function_contract\<close> where
+('s::sepalg, 'abort, 'i, 'o) striple_context \<Rightarrow>
+('e \<Rightarrow> ('s, 'f, 'abort, 'i prompt, 'o prompt_output) function_body) \<Rightarrow>
+('v \<Rightarrow> ('s, 'f, 'abort, 'i prompt, 'o prompt_output) function_body) \<Rightarrow>
+('s, 'f, 'abort) function_contract\<close> where
   [crush_contracts]: \<open>result_map_or_else_contract self pure_fun_def pure_fun \<Gamma> rust_fun_def rust_fun \<equiv>
     let pre  = \<langle>\<forall> i. \<Gamma>; rust_fun i \<Turnstile>\<^sub>F lift_pure_to_contract (pure_fun i)\<rangle> \<star>
                \<langle>\<forall> j. \<Gamma>; rust_fun_def j \<Turnstile>\<^sub>F lift_pure_to_contract (pure_fun_def j)\<rangle>;
         post = \<lambda>r. \<langle>r = (case self of Err(e) \<Rightarrow> pure_fun_def e | Ok(v) \<Rightarrow> pure_fun v)\<rangle>
     in make_function_contract pre post\<close>
 ucincl_auto result_map_or_else_contract
-
 
 lemma result_map_or_else_spec [crush_specs]:
   shows \<open>\<Gamma>; result_map_or_else self rust_fun_def rust_fun \<Turnstile>\<^sub>F 
@@ -877,10 +888,8 @@ ucincl_auto result_ok_contract
 
 lemma result_ok_spec [crush_specs]:
   shows \<open>\<Gamma>; result_ok res \<Turnstile>\<^sub>F result_ok_contract res\<close>
-  apply (crush_boot f: result_ok_def contract: result_ok_contract_def)
-  apply (cases res)
-  apply crush_base
-  done
+  by (crush_boot f: result_ok_def contract: result_ok_contract_def)
+     (crush_base split: result.splits)
 
 subsection\<open>or\<close>
 
@@ -914,15 +923,105 @@ ucincl_auto result_or_contract
 lemma result_or_spec [crush_specs]:
   shows \<open>\<Gamma>; result_or res if_err \<Turnstile>\<^sub>F result_or_contract res if_err\<close>
   by (crush_boot f: result_or_def contract: result_or_contract_def)
-     (crush_base simp add: result_or_pure_def split!: result.splits)
+     (crush_base simp add: result_or_pure_def split: result.splits)
 
 subsection\<open>or_else\<close>
 
+text\<open>Returns self if \<^verbatim>\<open>Result\<close> is of the \<^verbatim>\<open>Ok\<close> constructor, else applies the supplied function
+to the value of \<^verbatim>\<open>Err\<close> and returns a type \<^verbatim>\<open>Result\<close>.\<close>
+
+definition result_or_else :: \<open>('v, 'e) result \<Rightarrow>
+  ('e \<Rightarrow> ('s, ('v, 'e) result, 'abort, 'i, 'o) function_body) \<Rightarrow>
+  ('s, ('v, 'e) result, 'abort, 'i, 'o) function_body\<close> where
+  \<open>result_or_else self op \<equiv> FunctionBody \<lbrakk>
+    match self {
+      Ok(v)  \<Rightarrow> Ok(v),
+      Err(e) \<Rightarrow> op(e)
+    }
+  \<rbrakk>\<close>
+
+definition result_or_else_contract :: \<open>('v, 'e) result \<Rightarrow> ('e \<Rightarrow> ('v, 'e) result) \<Rightarrow> 
+('s::sepalg, 'abort, 'i, 'o) striple_context \<Rightarrow>
+('e \<Rightarrow> ('s, ('v, 'e) result, 'abort, 'i prompt, 'o prompt_output) function_body) \<Rightarrow>
+('s, ('v, 'e) result, 'abort) function_contract\<close> where
+  [crush_contracts]: \<open>result_or_else_contract self pure_fun \<Gamma> rust_fun \<equiv>
+    let pre  = \<langle>\<forall> i. \<Gamma>; rust_fun i \<Turnstile>\<^sub>F lift_pure_to_contract (pure_fun i)\<rangle>;
+        post = \<lambda>r. \<langle>r = (case self of Err(e) \<Rightarrow> pure_fun e | Ok(v) \<Rightarrow> Ok(v))\<rangle>
+    in make_function_contract pre post\<close>
+ucincl_auto result_or_else_contract
+
+lemma result_or_else_spec [crush_specs]:
+  shows \<open>\<Gamma>; result_or_else self rust_fun \<Turnstile>\<^sub>F result_or_else_contract self pure_fun \<Gamma> rust_fun\<close>
+proof (crush_boot f: result_or_else_def contract: result_or_else_contract_def, goal_cases)
+  case 1
+  note rust_fun_spec = this[THEN spec]
+  show ?case
+  proof (cases self)
+    case (Ok x1)
+    then show ?thesis by crush_base
+  next
+    case (Err x2)
+    then show ?thesis by (crush_base specs add: rust_fun_spec)
+  qed
+qed
+
 subsection\<open>transpose\<close>
+
+text\<open>Takes a type \<^verbatim>\<open>Result\<close> that matches either an \<^verbatim>\<open>Ok\<close> constructor
+ with a value of type \<^verbatim>\<open>Option\<close> or an \<^verbatim>\<open>Err\<close> constructor with any value. 
+Returns a type \<^verbatim>\<open>Option\<close> with a value of type \<^verbatim>\<open>Result\<close>, except in the case
+ where the input \<^verbatim>\<open>Option\<close> matched the \<^verbatim>\<open>None\<close> constructor, in which case returns \<^verbatim>\<open>None\<close>.
+Other than the \<^verbatim>\<open>None\<close> case, the value of the inner \<^verbatim>\<open>Option\<close> is transposed into the inner \<^verbatim>\<open>Result\<close>.\<close>
+
+definition result_transpose :: \<open>(('v) option, 'e) result \<Rightarrow>
+('s, (('v, 'e) result) option, 'abort, 'i, 'o) function_body\<close> where
+  \<open>result_transpose self \<equiv> FunctionBody \<lbrakk>
+    match self {
+      Ok(Some(x)) \<Rightarrow> Some(Ok(x)),
+      Ok(None) \<Rightarrow> None,
+      Err(e) \<Rightarrow> Some(Err(e))
+    }
+  \<rbrakk>\<close>
+
+definition result_transpose_contract :: \<open>(('v) option, 'e) result \<Rightarrow>
+  ('s::{sepalg}, (('v, 'e) result) option, 'abort) function_contract\<close> 
+  where [crush_contracts]: \<open>result_transpose_contract self \<equiv>
+    let pre  = UNIV;
+        post = \<lambda>r. \<langle>r = (case self of 
+          Ok(Some(x)) \<Rightarrow> Some(Ok(x)) |
+          Ok(None)    \<Rightarrow> None |
+          Err(e)      \<Rightarrow> Some(Err(e)) )\<rangle>
+    in make_function_contract pre post\<close>
+ucincl_auto result_transpose_contract
+
+lemma result_transpose_spec [crush_specs]:
+  shows \<open>\<Gamma>; result_transpose self \<Turnstile>\<^sub>F result_transpose_contract self\<close>
+proof (crush_boot f: result_transpose_def contract: result_transpose_contract_def, goal_cases)
+  case 1
+  then show ?case
+  proof (cases self)
+    case (Ok x1)
+    then show ?thesis 
+     proof (cases x1)
+       case None
+       with Ok show ?thesis by crush_base
+     next
+       case (Some a)
+       with Ok show ?thesis by crush_base
+     qed
+  next
+    case (Err x2)
+    then show ?thesis by crush_base
+  qed
+qed
+
+(*
+The above is left explicit for the reader, the Ok x1 can be proven by (cases x1; crush_base).
+*)
 
 subsection\<open>unwrap\<close>
 
-text\<open>Returns \<^verbatim>\<open>x\<close> if the element of \<^verbatim>\<open>Result\<close> type is of the form \<^verbatim>\<open>Ok x\<close>.  Panics otherwise.\<close>
+text\<open>Returns \<^verbatim>\<open>x\<close> if the element of type \<^verbatim>\<open>Result\<close> is of the form \<^verbatim>\<open>Ok x\<close>.  Panics otherwise.\<close>
 
 definition result_unwrap :: \<open>('v,'e) result \<Rightarrow> ('s, 'v, 'abort, 'i, 'o) function_body\<close> where
   \<open>result_unwrap self \<equiv> FunctionBody \<lbrakk>
@@ -940,18 +1039,44 @@ ucincl_auto result_unwrap_contract
 lemma result_unwrap_spec [crush_specs]:
   shows \<open>\<Gamma>; result_unwrap res \<Turnstile>\<^sub>F result_unwrap_contract res v\<close>
   by (crush_boot f: result_unwrap_def contract: result_unwrap_contract_def)
-     (crush_base split!: result.splits)
+     (crush_base split: result.splits)
 
 subsection\<open>unwrap_err\<close>
 
+text\<open>Returns \<^verbatim>\<open>x\<close> if the element of type \<^verbatim>\<open>Result\<close> is of form \<^verbatim>\<open>Err x\<close>, otherwise panics.\<close>
+
+definition result_unwrap_err :: \<open>('v, 'e) result \<Rightarrow> ('s, 'e, 'abort, 'i, 'o) function_body\<close> where
+  \<open>result_unwrap_err self \<equiv> FunctionBody \<lbrakk>
+    result_expect_err(self, "result_unwrap_err")
+  \<rbrakk>\<close>
+
+(*
+Note that should expect_err be added to the Core_Syntax consts, then the above could be refactored
+to match result_unwrap.
+*)
+
+definition result_unwrap_err_contract ::
+  \<open>('v, 'e) result \<Rightarrow> 'e \<Rightarrow> ('s::{sepalg}, 'e, 'abort) function_contract\<close>
+  where [crush_contracts]: \<open>result_unwrap_err_contract self e \<equiv>
+    let pre = \<langle>self = Err e\<rangle>; post = \<lambda>r. \<langle>r = e\<rangle>
+    in make_function_contract pre post\<close>
+ucincl_auto result_unwrap_err_contract
+
+lemma result_unwrap_err_spec [crush_specs]:
+  shows \<open>\<Gamma>; result_unwrap_err self \<Turnstile>\<^sub>F result_unwrap_err_contract self e\<close>
+  by (crush_boot f: result_unwrap_err_def contract: result_unwrap_err_contract_def)
+     (crush_base split: result.splits)
+
 subsection\<open>unwrap_err_unchecked\<close>
 
-subsection\<open>unrwrap_or\<close>
+text\<open>Unimplemented as this method is functionally identical to unwrap_err in µRust / HOL.\<close>
+
+subsection\<open>unwrap_or\<close>
 
 text\<open>Returns the \<^verbatim>\<open>Ok\<close> constructor of \<^verbatim>\<open>Result\<close> or the provided default, 
 dependant on the content of \<^verbatim>\<open>Result\<close>.\<close>
 
-definition result_unwrap_or :: \<open>('a, 'b) result \<Rightarrow> 'a \<Rightarrow> ('machine, 'a, 'abort, 'i prompt, 'o prompt_output) function_body\<close> where
+definition result_unwrap_or :: \<open>('a, 'b) result \<Rightarrow> 'a \<Rightarrow> ('s, 'a, 'abort, 'i prompt, 'o prompt_output) function_body\<close> where
   \<open>result_unwrap_or res e \<equiv> FunctionBody \<lbrakk>
      match res {
       Ok(r) \<Rightarrow> r,
@@ -968,16 +1093,57 @@ ucincl_auto result_unwrap_or_contract
 
 lemma result_unwrap_or_spec [crush_specs]:
   shows \<open>\<Gamma>; result_unwrap_or res e \<Turnstile>\<^sub>F result_unwrap_or_contract res e\<close>
-  apply (crush_boot f: result_unwrap_or_def contract: result_unwrap_or_contract_def)
-  apply (cases res)
-  apply crush_base
-  done
+  by (crush_boot f: result_unwrap_or_def contract: result_unwrap_or_contract_def)
+     (crush_base split: result.splits)
 
 subsection\<open>unwrap_or_default\<close>
 
+text\<open>Default values are not implemented for µRust types, therefore unwrap_or is the closest
+functional equivalent and should be used in place of unwrap_or_default.\<close>
+
 subsection\<open>unwrap_or_else\<close>
 
+text\<open>Returns the \<^verbatim>\<open>Ok\<close> value of \<^verbatim>\<open>Result\<close>, or applies the supplied function
+to the \<^verbatim>\<open>Err\<close> value and returns the result.\<close>
+
+definition result_unwrap_or_else :: \<open>('v, 'e) result \<Rightarrow> 
+  ('e \<Rightarrow> ('s, 'v, 'abort, 'i, 'o) function_body) \<Rightarrow>
+  ('s, 'v, 'abort, 'i, 'o) function_body\<close> where
+  \<open>result_unwrap_or_else self f \<equiv> FunctionBody \<lbrakk>
+    match self {
+      Ok(v)  \<Rightarrow> v,
+      Err(e) \<Rightarrow> f(e)
+    }
+  \<rbrakk>\<close>
+
+definition result_unwrap_or_else_contract :: \<open>('v, 'e) result \<Rightarrow> ('e \<Rightarrow> 'v) \<Rightarrow> 
+  ('s::sepalg, 'abort, 'i, 'o) striple_context \<Rightarrow>
+  ('e \<Rightarrow> ('s, 'v, 'abort, 'i prompt, 'o prompt_output) function_body) \<Rightarrow>
+  ('s, 'v, 'abort) function_contract\<close> where
+  [crush_contracts]: \<open>result_unwrap_or_else_contract self pure_fun \<Gamma> rust_fun \<equiv>
+    let pre  = \<langle>\<forall> i. \<Gamma>; rust_fun i \<Turnstile>\<^sub>F lift_pure_to_contract (pure_fun i)\<rangle>;
+        post = \<lambda>r. \<langle>r = (case self of Err(e) \<Rightarrow> pure_fun e | Ok(v) \<Rightarrow> v)\<rangle>
+    in make_function_contract pre post\<close>
+ucincl_auto result_unwrap_or_else_contract
+
+lemma result_unwrap_or_else_spec [crush_specs]:
+  shows \<open>\<Gamma>; result_unwrap_or_else self rust_fun \<Turnstile>\<^sub>F result_unwrap_or_else_contract self pure_fun \<Gamma> rust_fun\<close>
+proof (crush_boot f: result_unwrap_or_else_def contract: result_unwrap_or_else_contract_def, goal_cases)
+  case 1
+  note rust_fun_spec = this[THEN spec]
+  show ?case
+  proof (cases self)
+    case (Ok x1)
+    then show ?thesis by crush_base
+  next
+    case (Err x2)
+    then show ?thesis by (crush_base specs add: rust_fun_spec)
+  qed
+qed
+
 subsection\<open>unwrap_unchecked\<close>
+
+text\<open>Unimplemented as this method is functionally identical to unwrap in µRust / HOL.\<close>
 
 section\<open>Debug\<close>
 
